## 递归方程 ##

### - \\(f(n) = 6f(n-1)-8(n-2)\\) ; \\(f(1) = 1\\), \\(f(2) = 0\\) ###

求下面特征方程的解
$$ n^{2} - 6n + 8 = 0$$

得到 n = 2,4. 递归方程的通解：
$$f(n) = C1\*2^{n} + C2\*4^{n}$$   
根据初始条件   
\\(f(1) = C1\*2 + C2\*4 = 1\\)   
\\(f(2) = C1\*4 + C2\*16 = 0\\)   
得   
\\(C1 = 1\\)   
\\(C2 =-\frac{1}{4}\\)   
递归方程的特解：
$$f(n) =2^{n} - \frac{1}{4}\*4^{n} =  2^{n} -4^{n-1}$$ 

### - \\(f(n) = 5f(n-1)-6(n-2)\\) ;\\(f(1) = 1\\), \\(f(2) = 2\\)   ###

求下面特征方程的解
$$ n^{2} - 5n + 6 = 0$$

得到 n = 2,3. 递归方程的通解：
$$f(n) = C1\*2^{n} + C2\*3^{n}$$   
根据初始条件   
\\(f(1) = C1\*2 + C2\*3 = 1\\)   
\\(f(2) = C1\*4 + C2\*9 = 2\\)   
得   
\\(C1 = \frac{1}{2} \\)   
\\(C2 = 0\\)   
递归方程的特解：
$$f(n) =\frac{1}{2}\*2^{n} = 2^{n-1}$$ 


### - \\(f(n) = -6f(n-1)-9(n-2)\\) ;\\(f(1) = 3\\), \\(f(2) = 3\\)   ###

求下面特征方程的解
$$ n^{2} + 6n +9 = 0$$

得到 n = -3. 递归方程的通解：
$$f(n) = (A\*n \+ B)\*{(-3)}^{n}$$   
根据初始条件   
\\(f(1) = (A\+B)\*(-3) = 3\\)   
\\(f(2) = (2\* A\+B)\*9 = 3\\)   
得   
\\(A = \frac{4}{3} \\)   
\\(B = - \frac{7}{3} \\)  
递归方程的特解：
$$f(n) = (\frac{4}{3}\*n \- \frac{7}{3})\*{(-3)}^{n}$$   